Add frame_equalities in Steel framing subcomp

ulib/experimental/Steel.Effect.fst
@@ -406,42 +406,54 @@ let bind_opaque a b #framed_f #framed_g #pre_f #post_f #req_f #ens_f #pre_g #pos
 let bind a b #framed_f #framed_g #pre_f #post_f #req_f #ens_f #pre_g #post_g #req_g #ens_g #frame_f #frame_g #post #_ #_ #p #p2 f g
   = norm_repr (bind_opaque a b #framed_f #framed_g #pre_f #post_f #req_f #ens_f #pre_g #post_g #req_g #ens_g #frame_f #frame_g #post #_ #_ #p #p2 f g)
 
-/// Need to manually remove the rewrite_with_tactic marker here
-let lemma_unfold_subcomp_pre (#a:Type)
+unfold
+let subcomp_pre_opaque (#a:Type)
   (#pre_f:pre_t) (#post_f:post_t a) (req_f:req_t pre_f) (ens_f:ens_t pre_f a post_f)
   (#pre_g:pre_t) (#post_g:post_t a) (req_g:req_t pre_g) (ens_g:ens_t pre_g a post_g)
   (#frame:vprop)
-  (p1:squash (can_be_split pre_g (pre_f `star` frame)))
-  (p2:squash (equiv_forall post_g (fun x -> post_f x `star` frame)))
-  : Lemma
-  (requires subcomp_pre req_f ens_f req_g ens_g p1 p2)
-  (ensures (
-     can_be_split_trans pre_g (pre_f `star` frame) pre_f;
-     (forall (h0:hmem pre_g). req_g (mk_rmem pre_g h0) ==> req_f (focus_rmem (mk_rmem pre_g h0) pre_f)) /\
-     (forall (h0:hmem pre_g) (x:a) (h1:hmem (post_g x)). (
-        can_be_split_trans (post_g x) (post_f x `star` frame) (post_f x);
-        (req_g (mk_rmem pre_g h0) /\ ens_f (focus_rmem (mk_rmem pre_g h0) pre_f) x (focus_rmem (mk_rmem (post_g x) h1) (post_f x))) ==> ens_g (mk_rmem pre_g h0) x (mk_rmem (post_g x) h1)
-     ))
-  ))
-  = T.unfold_rewrite_with_tactic vc_norm (   can_be_split_trans pre_g (pre_f `star` frame) pre_f;
+  (_:squash (can_be_split pre_g (pre_f `star` frame)))
+  (_:squash (equiv_forall post_g (fun x -> post_f x `star` frame)))
+  : pure_pre
+= can_be_split_trans pre_g (pre_f `star` frame) pre_f;
   (forall (h0:hmem pre_g). req_g (mk_rmem pre_g h0) ==> req_f (focus_rmem (mk_rmem pre_g h0) pre_f)) /\
   (forall (h0:hmem pre_g) (x:a) (h1:hmem (post_g x)). (
      can_be_split_trans (post_g x) (post_f x `star` frame) (post_f x);
-     (req_g (mk_rmem pre_g h0) /\ ens_f (focus_rmem (mk_rmem pre_g h0) pre_f) x (focus_rmem (mk_rmem (post_g x) h1) (post_f x))) ==> ens_g (mk_rmem pre_g h0) x (mk_rmem (post_g x) h1)
-     ))
-  )
+     can_be_split_trans (pre_g) (pre_f `star` frame) frame;
+     can_be_split_trans (post_g x) (post_f x `star` frame) frame;
+
+     (req_g (mk_rmem pre_g h0) /\
+      ens_f (focus_rmem (mk_rmem pre_g h0) pre_f) x (focus_rmem (mk_rmem (post_g x) h1) (post_f x)) /\
+      frame_opaque frame
+        (focus_rmem (mk_rmem pre_g h0) frame)
+        (focus_rmem (mk_rmem (post_g x) h1) frame))
+
+        ==> ens_g (mk_rmem pre_g h0) x (mk_rmem (post_g x) h1)
+  ))
+
+val subcomp_opaque (a:Type)
+  (#framed_f:eqtype_as_type bool)
+  (#framed_g:eqtype_as_type bool)
+  (#[@@@ framing_implicit] pre_f:pre_t) (#[@@@ framing_implicit] post_f:post_t a)
+  (#[@@@ framing_implicit] req_f:req_t pre_f) (#[@@@ framing_implicit] ens_f:ens_t pre_f a post_f)
+  (#[@@@ framing_implicit] pre_g:pre_t) (#[@@@ framing_implicit] post_g:post_t a)
+  (#[@@@ framing_implicit] req_g:req_t pre_g) (#[@@@ framing_implicit] ens_g:ens_t pre_g a post_g)
+  (#[@@@ framing_implicit] frame:vprop)
+  (#[@@@ framing_implicit] _ : squash (maybe_emp framed_f frame))
+  (#[@@@ framing_implicit] p1:squash (can_be_split pre_g (pre_f `star` frame)))
+  (#[@@@ framing_implicit] p2:squash (equiv_forall post_g (fun x -> post_f x `star` frame)))
+  (f:repr a framed_f pre_f post_f req_f ens_f)
+: Pure (repr a framed_g pre_g post_g req_g ens_g)
+  (requires subcomp_pre_opaque req_f ens_f req_g ens_g p1 p2)
+  (ensures fun _ -> True)
 
 #push-options "--fuel 1 --ifuel 1 --z3rlimit 20"
 
-let subcomp a #framed_f #framed_g #pre_f #post_f #req_f #ens_f #pre_g #post_g #req_g #ens_g #fr #_ #p1 #p2 f =
+let subcomp_opaque a #framed_f #framed_g #pre_f #post_f #req_f #ens_f #pre_g #post_g #req_g #ens_g #fr #_ #p1 #p2 f =
   fun frame ->
     let m0 = nmst_get () in
     let h0 = mk_rmem pre_g (core_mem m0) in
-
-
     can_be_split_trans pre_g (pre_f `star` fr) pre_f;
-
-    lemma_unfold_subcomp_pre req_f ens_f req_g ens_g p1 p2;
+    can_be_split_trans pre_g (pre_f `star` fr) fr;
 
     can_be_split_3_interp (hp_of pre_g) (hp_of (pre_f `star` fr)) frame (locks_invariant Set.empty m0) m0;
 
@@ -452,7 +464,17 @@ let subcomp a #framed_f #framed_g #pre_f #post_f #req_f #ens_f #pre_g #post_g #r
     let m1 = nmst_get () in
     let h1 = mk_rmem (post_g x) (core_mem m1) in
 
+    let h0' = mk_rmem (pre_f `star` fr) (core_mem m0) in
+    let h1' = mk_rmem (post_f x `star` fr) (core_mem m1) in
+    // From frame00
+    assert (frame_opaque fr (focus_rmem h0' fr) (focus_rmem h1' fr));
+    // Replace h0'/h1' by h0/h1
+    focus_replace pre_g (pre_f `star` fr) fr (core_mem m0);
+    focus_replace (post_g x) (post_f x `star` fr) fr (core_mem m1);
+    assert (frame_opaque fr (focus_rmem h0 fr) (focus_rmem h1 fr));
+
     can_be_split_trans (post_g x) (post_f x `star` fr) (post_f x);
+    can_be_split_trans (post_g x) (post_f x `star` fr) fr;
 
     can_be_split_3_interp (hp_of (post_f x `star` fr)) (hp_of (post_g x)) frame (locks_invariant Set.empty m1) m1;
 
@@ -461,6 +483,141 @@ let subcomp a #framed_f #framed_g #pre_f #post_f #req_f #ens_f #pre_g #post_g #r
     x
 
 #pop-options
+
+let lemma_rewrite (p:Type) : Lemma (requires T.rewrite_with_tactic vc_norm p) (ensures p)
+  = T.unfold_rewrite_with_tactic vc_norm p
+
+let lemma_norm_opaque (p:Type) : Lemma (requires norm_opaque p) (ensures p) = ()
+
+(** Need to manually remove the rewrite_with_tactic marker here *)
+let lemma_subcomp_pre_opaque_aux1 (#a:Type)
+  (#pre_f:pre_t) (#post_f:post_t a) (req_f:req_t pre_f) (ens_f:ens_t pre_f a post_f)
+  (#pre_g:pre_t) (#post_g:post_t a) (req_g:req_t pre_g) (ens_g:ens_t pre_g a post_g)
+  (#frame:vprop)
+  (p1:squash (can_be_split pre_g (pre_f `star` frame)))
+  (p2:squash (equiv_forall post_g (fun x -> post_f x `star` frame)))
+  : Lemma
+  (requires subcomp_pre req_f ens_f req_g ens_g p1 p2)
+  (ensures  (can_be_split_trans pre_g (pre_f `star` frame) pre_f;
+    (forall (h0:hmem pre_g). req_g (mk_rmem pre_g h0) ==> req_f (focus_rmem (mk_rmem pre_g h0) pre_f)) /\
+    (forall (h0:hmem pre_g) (x:a) (h1:hmem (post_g x)). (
+
+     can_be_split_trans (post_g x) (post_f x `star` frame) (post_f x);
+     can_be_split_trans (pre_g) (pre_f `star` frame) frame;
+     can_be_split_trans (post_g x) (post_f x `star` frame) frame;
+
+     (req_g (mk_rmem pre_g h0) /\
+      ens_f (focus_rmem (mk_rmem pre_g h0) pre_f) x (focus_rmem (mk_rmem (post_g x) h1) (post_f x)) /\
+      frame_equalities frame
+        (focus_rmem (mk_rmem pre_g h0) frame)
+        (focus_rmem (mk_rmem (post_g x) h1) frame))
+
+        ==> ens_g (mk_rmem pre_g h0) x (mk_rmem (post_g x) h1)
+       ))))
+  = lemma_rewrite (squash (
+      can_be_split_trans pre_g (pre_f `star` frame) pre_f;
+      (forall (h0:hmem pre_g). req_g (mk_rmem pre_g h0) ==> req_f (focus_rmem (mk_rmem pre_g h0) pre_f)) /\
+      (forall (h0:hmem pre_g) (x:a) (h1:hmem (post_g x)). (
+         can_be_split_trans (post_g x) (post_f x `star` frame) (post_f x);
+         can_be_split_trans (pre_g) (pre_f `star` frame) frame;
+         can_be_split_trans (post_g x) (post_f x `star` frame) frame;
+
+         (req_g (mk_rmem pre_g h0) /\
+          ens_f (focus_rmem (mk_rmem pre_g h0) pre_f) x (focus_rmem (mk_rmem (post_g x) h1) (post_f x)) /\
+          frame_equalities frame
+            (focus_rmem (mk_rmem pre_g h0) frame)
+            (focus_rmem (mk_rmem (post_g x) h1) frame))
+
+            ==> ens_g (mk_rmem pre_g h0) x (mk_rmem (post_g x) h1)
+      ))
+    ))
+
+#push-options "--no_tactics"
+
+let lemma_subcomp_pre_opaque_aux2 (#a:Type)
+  (#pre_f:pre_t) (#post_f:post_t a) (req_f:req_t pre_f) (ens_f:ens_t pre_f a post_f)
+  (#pre_g:pre_t) (#post_g:post_t a) (req_g:req_t pre_g) (ens_g:ens_t pre_g a post_g)
+  (#frame:vprop)
+  (p1:squash (can_be_split pre_g (pre_f `star` frame)))
+  (p2:squash (equiv_forall post_g (fun x -> post_f x `star` frame)))
+  : Lemma
+ // (requires subcomp_pre req_f ens_f req_g ens_g p1 p2)
+  (requires  (can_be_split_trans pre_g (pre_f `star` frame) pre_f;
+    (forall (h0:hmem pre_g). req_g (mk_rmem pre_g h0) ==> req_f (focus_rmem (mk_rmem pre_g h0) pre_f)) /\
+    (forall (h0:hmem pre_g) (x:a) (h1:hmem (post_g x)). (
+
+     can_be_split_trans (post_g x) (post_f x `star` frame) (post_f x);
+     can_be_split_trans (pre_g) (pre_f `star` frame) frame;
+     can_be_split_trans (post_g x) (post_f x `star` frame) frame;
+
+     (req_g (mk_rmem pre_g h0) /\
+      ens_f (focus_rmem (mk_rmem pre_g h0) pre_f) x (focus_rmem (mk_rmem (post_g x) h1) (post_f x)) /\
+      frame_equalities frame
+        (focus_rmem (mk_rmem pre_g h0) frame)
+        (focus_rmem (mk_rmem (post_g x) h1) frame))
+
+        ==> ens_g (mk_rmem pre_g h0) x (mk_rmem (post_g x) h1)
+       ))))
+
+  (ensures subcomp_pre_opaque req_f ens_f req_g ens_g p1 p2)
+  = // T.unfold_rewrite_with_tactic vc_norm (squash (
+
+  //   can_be_split_trans pre_g (pre_f `star` frame) pre_f;
+  //   (forall (h0:hmem pre_g). req_g (mk_rmem pre_g h0) ==> req_f (focus_rmem (mk_rmem pre_g h0) pre_f)) /\
+  //   (forall (h0:hmem pre_g) (x:a) (h1:hmem (post_g x)). (
+
+  //    can_be_split_trans (post_g x) (post_f x `star` frame) (post_f x);
+  //    can_be_split_trans (pre_g) (pre_f `star` frame) frame;
+  //    can_be_split_trans (post_g x) (post_f x `star` frame) frame;
+
+  //    (req_g (mk_rmem pre_g h0) /\
+  //     ens_f (focus_rmem (mk_rmem pre_g h0) pre_f) x (focus_rmem (mk_rmem (post_g x) h1) (post_f x)) /\
+  //     frame_equalities frame
+  //       (focus_rmem (mk_rmem pre_g h0) frame)
+  //       (focus_rmem (mk_rmem (post_g x) h1) frame))
+
+  //       ==> ens_g (mk_rmem pre_g h0) x (mk_rmem (post_g x) h1)
+  //      ))
+  // ));
+  lemma_norm_opaque (squash (
+
+    can_be_split_trans pre_g (pre_f `star` frame) pre_f;
+    (forall (h0:hmem pre_g). req_g (mk_rmem pre_g h0) ==> req_f (focus_rmem (mk_rmem pre_g h0) pre_f)) /\
+    (forall (h0:hmem pre_g) (x:a) (h1:hmem (post_g x)). (
+
+     can_be_split_trans (post_g x) (post_f x `star` frame) (post_f x);
+     can_be_split_trans (pre_g) (pre_f `star` frame) frame;
+     can_be_split_trans (post_g x) (post_f x `star` frame) frame;
+
+     (req_g (mk_rmem pre_g h0) /\
+      ens_f (focus_rmem (mk_rmem pre_g h0) pre_f) x (focus_rmem (mk_rmem (post_g x) h1) (post_f x)) /\
+      frame_opaque frame
+        (focus_rmem (mk_rmem pre_g h0) frame)
+        (focus_rmem (mk_rmem (post_g x) h1) frame))
+
+        ==> ens_g (mk_rmem pre_g h0) x (mk_rmem (post_g x) h1)
+       ))
+  ))
+
+let lemma_subcomp_pre_opaque (#a:Type)
+  (#pre_f:pre_t) (#post_f:post_t a) (req_f:req_t pre_f) (ens_f:ens_t pre_f a post_f)
+  (#pre_g:pre_t) (#post_g:post_t a) (req_g:req_t pre_g) (ens_g:ens_t pre_g a post_g)
+  (#frame:vprop)
+  (p1:squash (can_be_split pre_g (pre_f `star` frame)))
+  (p2:squash (equiv_forall post_g (fun x -> post_f x `star` frame)))
+  : Lemma
+  (requires subcomp_pre req_f ens_f req_g ens_g p1 p2)
+  (ensures subcomp_pre_opaque req_f ens_f req_g ens_g p1 p2)
+  = lemma_subcomp_pre_opaque_aux1 req_f ens_f req_g ens_g p1 p2;
+    lemma_subcomp_pre_opaque_aux2 req_f ens_f req_g ens_g p1 p2
+
+#pop-options
+
+
+
+let subcomp a #framed_f #framed_g #pre_f #post_f #req_f #ens_f #pre_g #post_g #req_g #ens_g #fr #_ #p1 #p2 f =
+  lemma_subcomp_pre_opaque req_f ens_f req_g ens_g p1 p2;
+  subcomp_opaque a #framed_f #framed_g #pre_f #post_f #req_f #ens_f #pre_g #post_g #req_g #ens_g #fr #_ #p1 #p2 f
 
 let bind_pure_steel_ a b #wp #pre #post #req #ens f g
   = FStar.Monotonic.Pure.elim_pure_wp_monotonicity wp;
